Stash

src/examples/basic.lean
@@ -69,9 +69,15 @@ example (il : is_linear A) :
 end
 section
     universe u
-    variables {H G : Type u} [group H] [group G] {φ : H → G} {ψ : G → H} {x y z : G}
+    variables {H G : Type u} [group H] [group G] {φ : H → G} {ψ : G → H} {x y z h : G}
+    example : (x * z) * (z⁻¹ * y) = x * y
+    := by equate
     example : x * y = (x * z) * (z⁻¹ * y)
     := by equate
+    def conj (h x : G) := h * x * h ⁻¹ 
+    @[equate] lemma conj_def : conj h x = h * x * h ⁻¹ := rfl
+    example {h : G} : conj h (x) * conj h (y) = conj h (x * y) := by equate
+    example {h : G} : conj h (x * y) = conj h x * conj h y := by equate
     example : x * y⁻¹ = (y * x⁻¹)⁻¹
     := by equate
     example :  (y * x⁻¹)⁻¹ = x * y⁻¹
